Basalt/Examples/ArbChar.lean
@@ -6,50 +6,40 @@ open RandomChoice
 
 namespace ArbChar
 
-private theorem indexToChar_isAlphanum :
-    ∀ n, n ≤ 61 → (indexToChar n).isAlphanum = true := by decide
-
--- `decide` is too inefficient here, so we need to use `native_decide`
-private theorem isAlphanum_exists_index :
-    ∀ c : Char, c.isAlphanum = true → ∃ n, n ≤ 61 ∧ indexToChar n = c := by native_decide
+private theorem alphanumChars_eq_filter :
+    ∀ c : Char, c ∈ alphanumChars ↔ c.isAlphanum = true := by native_decide
 
 /-- All alphanumeric characters are generable by `Char.arbitrary` -/
 theorem Char.arbitrary_support :
     c ∈ SPMF.support Char.arbitrary ↔ c.isAlphanum = true := by
-  constructor
-  · -- c ∈ SPMF.support Char.arbitrary -> c.isAlphanum = true
-    intro h
-    rw [Char.arbitrary] at h
-    simp at h
-    obtain ⟨n, hle, rfl⟩ := h
-    apply indexToChar_isAlphanum
-    assumption
-  · -- c.isAlphanum = true -> c ∈ SPMF.support Char.arbitrary
-    intro h
-    rw [Char.arbitrary]
-    simp
-    obtain ⟨n, hhi, hc⟩ := isAlphanum_exists_index c h
-    exists n
-    constructor
-    . assumption
-    . apply hc.symm
+  rw [Char.arbitrary, SPMF.mem_support_elements_iff]
+  exact alphanumChars_eq_filter c
 
 /-- `Char.arbitrary` almost surely terminates -/
 theorem Char.arbitrary_terminates : SPMF.IsPMF Char.arbitrary := by
   unfold Char.arbitrary
-  apply SPMF.IsPMF_bind_pure
-  apply SPMF.IsPMF_choose
+  apply SPMF.IsPMF_elements
 
--- Proof is similar to `Nat.arbitrary_cost`, but `Char.arbitrary` makes only
--- one random choice, so `fun _ => 1` suffices as the cost function
 theorem Char.arbitrary_cost :
     IsBounded Char.arbitrary (fun _ => 1) := by
   rw [IsBounded_iff]
   rintro ⟨c, cost⟩ h
-  rw [Char.arbitrary] at h
-  simp [SPMF.Cost.mem_support_bind_iff, SPMF.Cost.mem_support_choose_iff,
-          SPMF.Cost.mem_support_pure_iff] at h
-  omega
+  rw [Char.arbitrary, elements] at h
+  simp only [SPMF.Cost.mem_support_bind_iff, Functor.map] at h
+  obtain ⟨⟨i, hi⟩, n1, n2, h1, h2, rfl⟩ := h
+  -- h2: (c, n2) ∈ support of (pure alphanumChars[i]) in Cost monad → n2 = 0
+  have hlen : alphanumChars.length = 62 := by native_decide
+  replace h2 : n2 = 0 := by
+    split at h2
+    simp only [Pure.pure, SPMF.mem_support_pure_iff, Prod.mk.injEq] at h2
+    exact h2.2
+  subst h2
+  -- h1: (⟨i,hi⟩, n1) ∈ support of (ULift.down <$> choose) in Cost monad → n1 = 1
+  replace h1 : n1 = 1 := by
+    revert h1
+    simp [SPMF.mem_support_bind_iff, SPMF.mem_support_pure_iff]
+  subst h1
+  simp
 
 #guard_msgs(drop info) in
 #eval (for _ in [0:20] do
